### 一些数论公式

- 当 $x\geq\phi(p)$ 时有 $a^x\equiv a^{x \; mod \; \phi(p) + \phi(p)}\pmod p$
- $\mu^2(n)=\sum_{d^2|n} \mu(d)$
- $\sum_{d|n} \varphi(d)=n$
- $\sum_{d|n} 2^{\omega(d)}=\sigma_0(n^2)$，其中 $\omega$ 是不同素因子个数
- $\sum_{d|n} \mu^2(d)=2^{\omega(d)}$

### 一些数论函数求和的例子

+ $\sum_{i=1}^n i[gcd(i, n)=1] = \frac {n \varphi(n) + [n=1]}{2}$
+ $\sum_{i=1}^n \sum_{j=1}^m [gcd(i,j)=x]=\sum_d \mu(d) \lfloor \frac n {dx} \rfloor  \lfloor \frac m {dx} \rfloor$
+ $\sum_{i=1}^n \sum_{j=1}^m gcd(i, j) = \sum_{i=1}^n \sum_{j=1}^m \sum_{d|gcd(i,j)} \varphi(d) = \sum_{d} \varphi(d) \lfloor \frac nd \rfloor \lfloor \frac md \rfloor$
+ $S(n)=\sum_{i=1}^n \mu(i)=1-\sum_{i=1}^n \sum_{d|i,d < i}\mu(d) \overset{t=\frac id}{=} 1-\sum_{t=2}^nS(\lfloor \frac nt \rfloor)$
    + 利用 $[n=1] = \sum_{d|n} \mu(d)$
+ $S(n)=\sum_{i=1}^n \varphi(i)=\sum_{i=1}^n i-\sum_{i=1}^n \sum_{d|i,d<i} \varphi(i)\overset{t=\frac id}{=} \frac {i(i+1)}{2} - \sum_{t=2}^n S(\frac n t)$
    + 利用 $n = \sum_{d|n} \varphi(d)$
+ $\sum_{i=1}^n \mu^2(i) = \sum_{i=1}^n \sum_{d^2|n} \mu(d)=\sum_{d=1}^{\lfloor \sqrt n \rfloor}\mu(d) \lfloor \frac n {d^2} \rfloor$ 
+ $\sum_{i=1}^n \sum_{j=1}^n gcd^2(i, j)= \sum_{d} d^2 \sum_{t} \mu(t) \lfloor \frac n{dt} \rfloor ^2 \\
    \overset{x=dt}{=} \sum_{x} \lfloor \frac nx \rfloor ^ 2 \sum_{d|x} d^2 \mu(\frac xd)$
+ $\sum_{i=1}^n \varphi(i)=\frac 12 \sum_{i=1}^n \sum_{j=1}^n [i \perp j] - 1=\frac 12 \sum_{i=1}^n \mu(i) \cdot\lfloor \frac n i \rfloor ^2-1$

### 斐波那契数列性质

- $F_{a+b}=F_{a-1} \cdot F_b+F_a \cdot F_{b+1}$
- $F_1+F_3+\dots +F_{2n-1} = F_{2n},F_2 + F_4 + \dots + F_{2n} = F_{2n + 1} - 1$
- $\sum_{i=1}^n F_i = F_{n+2} - 1$
- $\sum_{i=1}^n F_i^2 = F_n \cdot F_{n+1}$
- $F_n^2=(-1)^{n-1} + F_{n-1} \cdot F_{n+1}$
- $gcd(F_a, F_b)=F_{gcd(a, b)}$
- 模 $n$ 周期（皮萨诺周期）
    - $\pi(p^k) = p^{k-1} \pi(p)$
    - $\pi(nm) = lcm(\pi(n), \pi(m)), \forall n \perp m$
    - $\pi(2)=3, \pi(5)=20$
    - $\forall p \equiv \pm 1\pmod {10}, \pi(p)|p-1$
    - $\forall p \equiv \pm 2\pmod {5}, \pi(p)|2p+2$

### 常见生成函数

+ $(1+ax)^n=\sum_{k=0}^n \binom {n}{k} a^kx^k$
+ $\dfrac{1-x^{r+1}}{1-x}=\sum_{k=0}^nx^k$
+ $\dfrac1{1-ax}=\sum_{k=0}^{\infty}a^kx^k$
+ $\dfrac 1{(1-x)^2}=\sum_{k=0}^{\infty}(k+1)x^k$
+ $\dfrac1{(1-x)^n}=\sum_{k=0}^{\infty} \binom{n+k-1}{k}x^k$
+ $e^x=\sum_{k=0}^{\infty}\dfrac{x^k}{k!}$
+ $\ln(1+x)=\sum_{k=0}^{\infty}\dfrac{(-1)^{k+1}}{k}x^k$

